Rename mlkem_poly_{reduce,tomont,tobytes} -> mlkem_{...}
This avoids naming conflicts with mlkem-native when imported into AWS-LC.

Signed-off-by: Hanno Becker <beckphan@amazon.co.uk>

benchmarks/benchmark.c
@@ -832,9 +832,9 @@ void call_mlkem_basemul_k4(void) {}
 void call_mlkem_intt(void) {}
 void call_mlkem_mulcache_compute(void) {}
 void call_mlkem_ntt(void) {}
-void call_mlkem_poly_reduce(void) {}
-void call_mlkem_poly_tobytes(void) {}
-void call_mlkem_poly_tomont(void) {}
+void call_mlkem_reduce(void) {}
+void call_mlkem_tobytes(void) {}
+void call_mlkem_tomont(void) {}
 void call_mlkem_rej_uniform(void) {}
 void call_sha3_keccak_f1600(void) {}
 void call_sha3_keccak_f1600_alt(void) {}
@@ -1126,9 +1126,9 @@ void call_mlkem_basemul_k4(void) repeat(mlkem_basemul_k4((int16_t*)b0,(int16_t*)
 void call_mlkem_intt(void) repeat(mlkem_intt((int16_t*)b0,(int16_t*)b1,(int16_t*)b2))
 void call_mlkem_mulcache_compute(void) repeat(mlkem_mulcache_compute((int16_t*)b0,(int16_t*)b1,(int16_t*)b2,(int16_t*)b3))
 void call_mlkem_ntt(void) repeat(mlkem_ntt((int16_t*)b0,(int16_t*)b1,(int16_t*)b2))
-void call_mlkem_poly_reduce(void) repeat(mlkem_poly_reduce((int16_t*)b0))
-void call_mlkem_poly_tobytes(void) repeat(mlkem_poly_tobytes((uint8_t*)b0,(int16_t*)b1))
-void call_mlkem_poly_tomont(void) repeat(mlkem_poly_tomont((int16_t*)b0))
+void call_mlkem_reduce(void) repeat(mlkem_reduce((int16_t*)b0))
+void call_mlkem_tobytes(void) repeat(mlkem_tobytes((uint8_t*)b0,(int16_t*)b1))
+void call_mlkem_tomont(void) repeat(mlkem_tomont((int16_t*)b0))
 void call_mlkem_rej_uniform(void) repeat(mlkem_rej_uniform_VARIABLE_TIME((int16_t*)b0,(uint8_t*)b1,1200,mlkem_rej_uniform_table))
 void call_sha3_keccak_f1600(void) repeat(sha3_keccak_f1600(b0,b1))
 void call_sha3_keccak_f1600_alt(void) repeat(sha3_keccak_f1600_alt(b0,b1))
@@ -1525,9 +1525,9 @@ int main(int argc, char *argv[])
   timingtest(arm,"mlkem_intt",call_mlkem_intt);
   timingtest(arm,"mlkem_mulcache_compute",call_mlkem_mulcache_compute);
   timingtest(arm,"mlkem_ntt",call_mlkem_ntt);
-  timingtest(arm,"mlkem_poly_reduce",call_mlkem_poly_reduce);
-  timingtest(arm,"mlkem_poly_tobytes",call_mlkem_poly_tobytes);
-  timingtest(arm,"mlkem_poly_tomont",call_mlkem_poly_tomont);
+  timingtest(arm,"mlkem_reduce",call_mlkem_reduce);
+  timingtest(arm,"mlkem_tobytes",call_mlkem_tobytes);
+  timingtest(arm,"mlkem_tomont",call_mlkem_tomont);
   timingtest(arm,"mlkem_rej_uniform_VARIABLE_TIME (1200 bytes)",call_mlkem_rej_uniform);
   timingtest(bmi,"p256_montjadd",call_p256_montjadd);
   timingtest(all,"p256_montjadd_alt",call_p256_montjadd_alt);
