include/s2n-bignum.h
@@ -1004,15 +1004,15 @@ extern void mlkem_ntt(int16_t a[S2N_BIGNUM_STATIC 256],const int16_t z_01234[S2N
 
 // Canonical modular reduction of polynomial coefficients for ML-KEM
 // Input a[256] (signed 16-bit words); output a[256] (signed 16-bit words)
-extern void mlkem_poly_reduce(int16_t a[S2N_BIGNUM_STATIC 256]);
+extern void mlkem_reduce(int16_t a[S2N_BIGNUM_STATIC 256]);
 
 // Pack ML-KEM polynomial coefficients as 12-bit numbers
 // Input a[256] (signed 16-bit words); output r[384] (bytes)
-extern void mlkem_poly_tobytes(uint8_t r[S2N_BIGNUM_STATIC 384],const int16_t a[S2N_BIGNUM_STATIC 256]);
+extern void mlkem_tobytes(uint8_t r[S2N_BIGNUM_STATIC 384],const int16_t a[S2N_BIGNUM_STATIC 256]);
 
 // Conversion of ML-KEM polynomial coefficients to Montgomery form
 // Input a[256] (signed 16-bit words); output a[256] (signed 16-bit words)
-extern void mlkem_poly_tomont(int16_t a[S2N_BIGNUM_STATIC 256]);
+extern void mlkem_tomont(int16_t a[S2N_BIGNUM_STATIC 256]);
 
 // Uniform rejection sampling for ML-KEM
 // Inputs *buf (unsigned bytes), buflen, table (unsigned bytes); output r[256] (signed 16-bit words), return
